src/mcl/ts_updates.lean
@@ -12,7 +12,7 @@ inductive op (sig : signature)
 | store {t} {dim} (var : string) (idx : vector (expression sig type.int) dim) (h₁ : type_of (sig.val var) = t) (h₂ : ((sig.val var).type).dim = dim) : op
 | compute_list (computes : list (memory (parlang_mcl_tlocal sig) → memory (parlang_mcl_tlocal sig))) : op
 
-def ts_updates {sig : signature} : list (op sig) → thread_state (memory $ parlang_mcl_tlocal sig) (parlang_mcl_global sig) → thread_state (memory $ parlang_mcl_tlocal sig) (parlang_mcl_global sig)
+def ts_updates {sig : signature} : list (op sig) → thread_state (memory $ parlang_mcl_tlocal sig) (parlang_mcl_shared sig) → thread_state (memory $ parlang_mcl_tlocal sig) (parlang_mcl_shared sig)
 | [] ts := ts
 | (op.store var idx h₁ h₂ :: ops) ts := ts_updates ops $ mcl_store var idx h₁ h₂ ts
 | (op.compute_list computes :: ops) ts := ts_updates ops $ compute_list computes ts
@@ -33,24 +33,24 @@ lemma ts_update_split {sig : signature} (up) (ups : list (op sig)) : ts_updates 
     }
 end
 
-lemma ts_updates_tlocal {sig : signature}  {ts : thread_state (memory $ parlang_mcl_tlocal sig) (parlang_mcl_global sig)} {updates} (m loads stores) : 
-(ts_updates updates ts).tlocal = (ts_updates updates { tlocal := ts.tlocal, loads := loads, stores := stores, global := m }).tlocal := begin
+lemma ts_updates_tlocal {sig : signature}  {ts : thread_state (memory $ parlang_mcl_tlocal sig) (parlang_mcl_shared sig)} {updates} (m loads stores) : 
+(ts_updates updates ts).tlocal = (ts_updates updates { tlocal := ts.tlocal, loads := loads, stores := stores, shared := m }).tlocal := begin
     sorry,
 end
 
-lemma ts_updates_nil {sig : signature} (f : thread_state (memory $ parlang_mcl_tlocal sig) (parlang_mcl_global sig) → thread_state (memory $ parlang_mcl_tlocal sig) (parlang_mcl_global sig)) : 
+lemma ts_updates_nil {sig : signature} (f : thread_state (memory $ parlang_mcl_tlocal sig) (parlang_mcl_shared sig) → thread_state (memory $ parlang_mcl_tlocal sig) (parlang_mcl_shared sig)) : 
 ts_updates [] ∘ f = f := begin
     refl,
 end
 
 @[simp]
-lemma ts_updates_store {sig : signature} {dim} {idx : vector (expression sig type.int) dim} {var t} {h₁ : type_of (sig.val var) = t} {h₂} {updates} (f : thread_state (memory $ parlang_mcl_tlocal sig) (parlang_mcl_global sig) → thread_state (memory $ parlang_mcl_tlocal sig) (parlang_mcl_global sig)) : 
+lemma ts_updates_store {sig : signature} {dim} {idx : vector (expression sig type.int) dim} {var t} {h₁ : type_of (sig.val var) = t} {h₂} {updates} (f : thread_state (memory $ parlang_mcl_tlocal sig) (parlang_mcl_shared sig) → thread_state (memory $ parlang_mcl_tlocal sig) (parlang_mcl_shared sig)) : 
 ts_updates updates ∘ mcl_store var idx h₁ h₂ ∘ f = ts_updates (op.store var idx h₁ h₂ :: updates) ∘ f := begin
     refl,
 end
 
 @[simp]
-lemma ts_updates_compute {sig : signature} {g} {updates} (f : thread_state (memory $ parlang_mcl_tlocal sig) (parlang_mcl_global sig) → thread_state (memory $ parlang_mcl_tlocal sig) (parlang_mcl_global sig)) : 
+lemma ts_updates_compute {sig : signature} {g} {updates} (f : thread_state (memory $ parlang_mcl_tlocal sig) (parlang_mcl_shared sig) → thread_state (memory $ parlang_mcl_tlocal sig) (parlang_mcl_shared sig)) : 
 ts_updates updates ∘ compute g ∘ f = ts_updates (op.compute_list [g] :: updates) ∘ f := begin
     refl,
 end
@@ -63,7 +63,7 @@ end
 
 @[simp]
 lemma compute_list_stores' {sig : signature} {n} {tid : fin n} {ac : vector bool n} {computes}
-{s : state n (memory $ parlang_mcl_tlocal sig) (parlang_mcl_global sig)} : 
+{s : state n (memory $ parlang_mcl_tlocal sig) (parlang_mcl_shared sig)} : 
 (vector.nth ((map_active_threads ac (ts_updates [op.compute_list computes]) s).threads) tid).stores = (vector.nth s.threads tid).stores := begin
     by_cases h : ac.nth tid = tt,
     {
@@ -75,7 +75,7 @@ end
 
 @[simp]
 lemma compute_list_loads' {sig : signature} {n} {tid : fin n} {ac : vector bool n} {computes}
-{s : state n (memory $ parlang_mcl_tlocal sig) (parlang_mcl_global sig)} : 
+{s : state n (memory $ parlang_mcl_tlocal sig) (parlang_mcl_shared sig)} : 
 (vector.nth ((map_active_threads ac (ts_updates [op.compute_list computes]) s).threads) tid).loads = (vector.nth s.threads tid).loads := begin
     by_cases h : ac.nth tid = tt,
     {
@@ -87,8 +87,8 @@ end
 
 @[simp]
 lemma compute_list_shared' {sig : signature} {n} {tid : fin n} {ac : vector bool n} {computes}
-{s : state n (memory $ parlang_mcl_tlocal sig) (parlang_mcl_global sig)} : 
-(vector.nth ((map_active_threads ac (ts_updates [op.compute_list computes]) s).threads) tid).global = (vector.nth s.threads tid).global := begin
+{s : state n (memory $ parlang_mcl_tlocal sig) (parlang_mcl_shared sig)} : 
+(vector.nth ((map_active_threads ac (ts_updates [op.compute_list computes]) s).threads) tid).shared = (vector.nth s.threads tid).shared := begin
     by_cases h : ac.nth tid = tt,
     {
         simp [ts_updates, map_active_threads_nth_ac h],
