src/use_cases/arrcp_mcl.lean
@@ -13,25 +13,25 @@ namespace arrcp_mcl
 #check ([5] : vector _ _)
 
 
-def sig : signature --:= λ n, if n = "i" then { scope := scope.tlocal, type := ⟨_, [1], type.int⟩ } else { scope := scope.global, type := ⟨_, [100], type.int⟩ }
+def sig : signature --:= λ n, if n = "i" then { scope := scope.tlocal, type := ⟨_, [1], type.int⟩ } else { scope := scope.shared, type := ⟨_, [100], type.int⟩ }
 | "i" := { scope := scope.tlocal, type := ⟨_, [1], type.int⟩ }
 | "tid" := { scope := scope.tlocal, type := ⟨_, [1], type.int⟩ }
-| _ := { scope := scope.global, type := ⟨_, [100], type.int⟩ }
+| _ := { scope := scope.shared, type := ⟨_, [100], type.int⟩ }
 
 lemma i_is_tlocal : is_tlocal (sig "i") := by apply eq.refl
-lemma a_is_global : is_global (sig "a") := by apply eq.refl
+lemma a_is_shared : is_shared (sig "a") := by apply eq.refl
 lemma tid_is_tlocal : is_tlocal (sig "tid") := by apply eq.refl
 
 def read_i := (expression.tlocal_var "i" (λ_, 0) (show type_of (sig "i") = type.int, by apply eq.refl) (by refl) i_is_tlocal)
 def read_tid := (expression.tlocal_var "tid" (λ_, 0) (show type_of (sig "tid") = type.int, by apply eq.refl) (show (sig "tid").type.dim = 1, by apply eq.refl) tid_is_tlocal)
 
 def arrcp₁ : mclp sig := mclp.intro (λ m, 100) (
-    mclk.global_assign "b" [read_tid] (by refl) (expression.global_var "a" (λ_, read_tid) (show type_of (sig "a") = type.int, by refl) (by refl) a_is_global)
+    mclk.shared_assign "b" [read_tid] (by refl) (expression.shared_var "a" (λ_, read_tid) (show type_of (sig "a") = type.int, by refl) (by refl) a_is_shared)
 )
 
 
 def arrcp₂ : mclp sig := mclp.intro (λ m, 10) (mclk.for "i" (by refl) (by refl) read_tid (read_i < 100) (mclk.tlocal_assign "i" [1] (show ((sig "i").type).dim = vector.length [1], by refl) (read_i + read_tid)) (
-    mclk.global_assign "b" [read_i] (by refl) (expression.global_var "a" (λ_, read_i) (show type_of (sig "a") = type.int, by refl) (by refl) a_is_global)
+    mclk.shared_assign "b" [read_i] (by refl) (expression.shared_var "a" (λ_, read_i) (show type_of (sig "a") = type.int, by refl) (by refl) a_is_shared)
 ))
 
 #eval mclp_to_program arrcp₁
@@ -40,7 +40,7 @@ def arrcp₂ : mclp sig := mclp.intro (λ m, 10) (mclk.for "i" (by refl) (by ref
 
 example (c) : mclp_to_program arrcp₁ = c := begin
     rw arrcp₁,
-    rw [mclp_to_program, mclk_to_kernel, prepend_load_expr, load_global_vars_for_expr],
+    rw [mclp_to_program, mclk_to_kernel, prepend_load_expr, load_shared_vars_for_expr],
     repeat {rw list.append},
     repeat {rw list.foldl},
     repeat {rw list.foldr},
