src/mcl/compute_list.lean
@@ -23,13 +23,13 @@ lemma compute_list_merge {σ ι : Type} {τ : ι → Type} [decidable_eq ι] (f 
     }
 end
 
-lemma compute_list_accesses {sig : signature} {n} (s : state n (memory $ parlang_mcl_tlocal sig) (parlang_mcl_global sig)) (i) (computes) (tid) : 
+lemma compute_list_accesses {sig : signature} {n} (s : state n (memory $ parlang_mcl_tlocal sig) (parlang_mcl_shared sig)) (i) (computes) (tid) : 
 i ∉ (compute_list computes (vector.nth (s.threads) tid)).accesses ↔ i ∉ (vector.nth (s.threads) tid).accesses := sorry
 
 -- todo: rewrite to s = { tlocal := ... s.tlocal, ..s }
-lemma compute_list_tlocal {sig : signature} {computes : list (memory (parlang_mcl_tlocal sig) → memory (parlang_mcl_tlocal sig))} {tlocal loads stores} {global : memory $ parlang_mcl_global sig} : 
-compute_list computes {tlocal := tlocal, global := global, loads := loads, stores := stores} = 
-{tlocal := computes.foldl (λ tl com, com tl) tlocal, global := global, loads := loads, stores := stores} := begin
+lemma compute_list_tlocal {sig : signature} {computes : list (memory (parlang_mcl_tlocal sig) → memory (parlang_mcl_tlocal sig))} {tlocal loads stores} {shared : memory $ parlang_mcl_shared sig} : 
+compute_list computes {tlocal := tlocal, shared := shared, loads := loads, stores := stores} = 
+{tlocal := computes.foldl (λ tl com, com tl) tlocal, shared := shared, loads := loads, stores := stores} := begin
     induction computes generalizing tlocal,
     {
         refl,
@@ -40,7 +40,7 @@ end
 
 @[simp]
 lemma compute_list_stores_core {sig : signature} {computes}
-{ts : thread_state (memory $ parlang_mcl_tlocal sig) (parlang_mcl_global sig)} : 
+{ts : thread_state (memory $ parlang_mcl_tlocal sig) (parlang_mcl_shared sig)} : 
 (compute_list computes ts).stores = ts.stores := begin
     induction computes generalizing ts,
     { simp [compute_list], },
@@ -49,7 +49,7 @@ end
 
 @[simp]
 lemma compute_list_loads_core {sig : signature} {computes}
-{ts : thread_state (memory $ parlang_mcl_tlocal sig) (parlang_mcl_global sig)} : 
+{ts : thread_state (memory $ parlang_mcl_tlocal sig) (parlang_mcl_shared sig)} : 
 (compute_list computes ts).loads = ts.loads := begin
     induction computes generalizing ts,
     { simp [compute_list], },
@@ -58,17 +58,17 @@ end
 
 @[simp]
 lemma compute_list_shared {sig : signature} {computes}
-{ts : thread_state (memory $ parlang_mcl_tlocal sig) (parlang_mcl_global sig)} : 
-(compute_list computes ts).global = ts.global := begin
+{ts : thread_state (memory $ parlang_mcl_tlocal sig) (parlang_mcl_shared sig)} : 
+(compute_list computes ts).shared = ts.shared := begin
     induction computes generalizing ts,
     { simp [compute_list], },
     { cases ts, simp [compute_list, compute], rw computes_ih, },
 end
 
 lemma compute_list_stores {sig : signature} {computes}
-{ts : thread_state (memory $ parlang_mcl_tlocal sig) (parlang_mcl_global sig)} {i : mcl_address sig} : 
+{ts : thread_state (memory $ parlang_mcl_tlocal sig) (parlang_mcl_shared sig)} {i : mcl_address sig} : 
 i ∉ ts.stores ↔ i ∉ (compute_list computes ts).stores := by simp
 
 lemma compute_list_loads {sig : signature} {computes}
-{ts : thread_state (memory $ parlang_mcl_tlocal sig) (parlang_mcl_global sig)} {i : mcl_address sig} : 
+{ts : thread_state (memory $ parlang_mcl_tlocal sig) (parlang_mcl_shared sig)} {i : mcl_address sig} : 
 i ∉ ts.loads ↔ i ∉ (compute_list computes ts).loads := by simp
