src/use_cases/assign_mcl.lean
@@ -16,7 +16,7 @@ open parlang.state
 open parlang.thread_state
 
 /- not in use -/
--- lemma store_access_elim_name {sig : signature} {n n_idx} {s : state n (memory $ parlang_mcl_tlocal sig) (parlang_mcl_global sig)} {var} {idx : vector (expression sig type.int) n_idx} 
+-- lemma store_access_elim_name {sig : signature} {n n_idx} {s : state n (memory $ parlang_mcl_tlocal sig) (parlang_mcl_shared sig)} {var} {idx : vector (expression sig type.int) n_idx} 
 -- {t h₄} {h₃ : type_of (sig.val var) = t } {f} {t : fin n} {i} {ac₁ : vector bool n} {updates}
 -- (h₁ : i ∉ accesses (vector.nth ((map_active_threads ac₁ (f ∘ compute_list updates) s).threads) t)) 
 -- (h₂ : i.1 ≠ var) :
@@ -25,9 +25,9 @@ open parlang.thread_state
 -- end
 
 -- lemma store_no_stores_name {sig : signature} {dim} {idx : vector (expression sig type.int) dim} {var t} {h₁ : type_of (sig.val var) = t} {h₂} {computes : list (memory (parlang_mcl_tlocal sig) → memory (parlang_mcl_tlocal sig))}
--- {ts : thread_state (memory $ parlang_mcl_tlocal sig) (parlang_mcl_global sig)} {i : mcl_address sig}
--- {n} {s : state n (memory $ parlang_mcl_tlocal sig) (parlang_mcl_global sig)} {m : memory (parlang_mcl_global sig)} {tid}
--- {f : thread_state (memory $ parlang_mcl_tlocal sig) (parlang_mcl_global sig) → thread_state (memory $ parlang_mcl_tlocal sig) (parlang_mcl_global sig)} : 
+-- {ts : thread_state (memory $ parlang_mcl_tlocal sig) (parlang_mcl_shared sig)} {i : mcl_address sig}
+-- {n} {s : state n (memory $ parlang_mcl_tlocal sig) (parlang_mcl_shared sig)} {m : memory (parlang_mcl_shared sig)} {tid}
+-- {f : thread_state (memory $ parlang_mcl_tlocal sig) (parlang_mcl_shared sig) → thread_state (memory $ parlang_mcl_tlocal sig) (parlang_mcl_shared sig)} : 
 -- syncable ((f ∘ compute_list computes) s) m →
 -- i.fst ≠ var →
 -- i ∉ ((f ∘ compute_list computes) (s.threads.nth tid)).stores →
